verify/LongLoop.v
@@ -1,0 +1,2417 @@
+From BusyCoq Require Import Individual62.
+
+Require Import ZifyN Lia.
+Require Import ZArith.
+Require Import List.
+Import Eqb.
+
+Open Scope N.
+
+Definition Nsubge(a b:N) :=
+if b <=? a then Some (a-b) else None.
+
+Lemma Nsubge_spec a b c:
+  Nsubge a b = Some c ->
+  a=c+b.
+Proof.
+  unfold Nsubge.
+  intros.
+  destruct (N.leb_spec b a);
+  inverts H; lia.
+Qed.
+
+Definition Ndiv(a b:N) :=
+if a mod b =? 0 then Some (a/b) else None.
+
+Lemma Ndiv_spec a b c:
+  Ndiv a b = Some c ->
+  a=c*b.
+Proof.
+  unfold Ndiv.
+  intros.
+  destruct (N.eqb_spec (a mod b) 0);
+  inverts H.
+  pose proof (N.div_mod a b); lia.
+Qed.
+
+Definition N_OS(n:N) :=
+match n with
+| N0 => None
+| _ => Some (N.pred n)
+end.
+
+Lemma N_OS_spec n:
+(match N_OS n with
+| None => n=N0
+| Some n0 => n=1+n0
+end)%N.
+Proof.
+  unfold N_OS.
+  destruct n; lia.
+Qed.
+
+Definition if_None {A} (a:option A) b :=
+match a with
+| None => b tt
+| _ => a
+end.
+
+Notation "a ||| b" := (if_None a b) (at level 30, right associativity).
+
+Definition b2o(b:bool) := if b then Some tt else None.
+
+Notation seg := (list Sym).
+Notation head := (DH0*DH0)%type.
+Notation vseg := (list seg + list seg)%type.
+Notation vside := (list vseg * seg)%type.
+
+Ltac ec := econstructor.
+Ltac eex := repeat eexists.
+
+Ltac des_if H :=
+  cbn[if_None] in H;
+  cbn[if_Some] in H;
+  let E:=fresh "E" in
+  match type of H with
+  | ?a ||| _ = _ =>
+    destruct a eqn:E
+  | ?a &&& _ = _ =>
+    destruct a eqn:E
+  end.
+
+Ltac des_if' H := des_if H; [|inverts H].
+
+
+Section sec.
+Hypothesis f2:seg->head->option(N*N*head).
+Hypothesis f1:seg->head->option((list seg)*(list head)).
+Hypothesis f0:seg->head->option((list seg)*seg).
+Hypothesis tm:TM.
+
+Definition to_side '(ws,w) :=
+  concat ws*>w*>0inf.
+
+Hypothesis f2_spec:
+  forall w h a0 a1 h',
+  f2 w h = Some (a0,a1,h') ->
+  segRLs tm ([h]^^(N.to_nat (2^a0))) ([h']^^(N.to_nat (2^a1))) w w.
+
+Hypothesis f1_spec:
+  forall w h ws hs,
+  f1 w h = Some (ws,hs) ->
+  segRLs tm [h] hs w (concat ws).
+
+Hypothesis f0_spec:
+  forall w h w',
+  f0 w h = Some w' ->
+  sideRLs tm [h] (w*>0inf) (to_side w').
+
+Inductive Nmap :=
+| Nmap_mk(a0 a1 b0 b1:N)
+| Nmap_c(b0 b1:N).
+
+Inductive Nmap_apply: Nmap->N->N->Prop :=
+| Nmap_apply_mk(a0 a1 b0 b1 n:N): Nmap_apply (Nmap_mk a0 a1 b0 b1) (2^a0*n+b0) (2^a1*n+b1)
+| Nmap_apply_c b0 b1: Nmap_apply (Nmap_c b0 b1) b0 b1.
+
+Inductive vN :=
+| vN_v(id:N)(mp:Nmap)
+| vN_c(c:N).
+
+Definition Nmap_add x k :=
+match x with
+| Nmap_mk a0 a1 b0 b1 => Nmap_mk a0 a1 b0 (b1+k)
+| Nmap_c b0 b1 => Nmap_c b0 (b1+k)
+end.
+
+Definition vN_add a b :=
+match a,b with
+| vN_c a,vN_c b => Some (vN_c (a+b))
+| vN_c a,vN_v id mp => Some (vN_v id (Nmap_add mp a))
+| vN_v id mp,vN_c b => Some (vN_v id (Nmap_add mp b))
+| _,_ => None
+end.
+
+Inductive vhead :=
+| vhead_mk(h:head)(n:N)(n':vN)
+.
+
+Section vhead_sec.
+Hypothesis ctx:N->N.
+Inductive vN_eval: vN->N->Prop :=
+| vN_eval_v id mp n:
+  Nmap_apply mp (ctx id) n ->
+  vN_eval (vN_v id mp) n
+| vN_eval_c c:
+  vN_eval (vN_c c) c.
+
+Inductive vhead_eval: vhead -> list head -> Prop :=
+| vhead_eval_mk h n n' n'0:
+  vN_eval n' n'0 ->
+  vhead_eval (vhead_mk h n n') ([h]^^(N.to_nat n'0)).
+
+Inductive vheads_eval: list vhead -> list head -> Prop :=
+| vheads_eval_O: vheads_eval [] []
+| vheads_eval_S h t h' t':
+  vhead_eval h h' ->
+  vheads_eval t t' ->
+  vheads_eval (h::t) (h'++t').
+
+Inductive Nmap_applys: Nmap->N->N->N->Prop :=
+| Nmap_applys_O mp n: Nmap_applys mp n n 0
+| Nmap_applys_S mp n n0 n1 k:
+  Nmap_apply mp n n0 ->
+  Nmap_applys mp n0 n1 k ->
+  Nmap_applys mp n n1 (1+k).
+
+Inductive vN_evaln: vN->N->N->Prop :=
+| vN_evaln_v id mp n i:
+  Nmap_applys mp (ctx id) n i ->
+  vN_evaln (vN_v id mp) n i
+| vN_evaln_c c i:
+  vN_evaln (vN_c c) c i.
+
+Inductive vhead_evaln: vhead -> list head -> N -> Prop :=
+| vhead_evaln_mk h n n' n'0 i:
+  vN_evaln n' n'0 i ->
+  vhead_evaln (vhead_mk h n n') ([h]^^(N.to_nat n'0)) i.
+
+Inductive vheads_evaln: list vhead -> list head -> N -> Prop :=
+| vheads_evaln_O n: vheads_evaln [] [] n
+| vheads_evaln_S h t h' t' n:
+  vhead_evaln h h' n ->
+  vheads_evaln t t' n ->
+  vheads_evaln (h::t) (h'++t') n.
+
+Definition vhead_add a b :=
+match a,b with
+| vhead_mk h n n',vhead_mk h0 n0 n'0 =>
+  b2o (eqb h h0) &&& (fun _ =>
+  vN_add n' n'0 &&& (fun n'1 =>
+  Some (vhead_mk h (n+n0) n'1)))
+end.
+
+Definition vN_is0' n :=
+match n with
+| vN_c c => b2o (c=?0)
+| _ => None
+end.
+
+Definition vN_is0 n :=
+match n with
+| vN_c c => b2o (c=?0)
+| vN_v _ (Nmap_c b0 b1) => b2o (b1=?0)
+| _ => None
+end.
+
+Definition vhead_is0' x :=
+match x with
+| vhead_mk h n n' => vN_is0' n'
+end.
+
+Fixpoint vheads_simpl(ls ls0:list vhead) :=
+match ls with
+| h::t =>
+  if vhead_is0' h then vheads_simpl t ls0 else
+  match vheads_simpl t ls0 with
+  | [] => [h]
+  | h0::t0 =>
+    match vhead_add h h0 with
+    | Some h1 => h1::t0
+    | None => h::h0::t0
+    end
+  end
+| [] => ls0
+end.
+
+Definition Nmap_sub x k :=
+match x with
+| Nmap_mk a0 a1 b0 b1 =>
+  let c:=(k-b1+(2^a1-1))/2^a1 in
+  Some (Nmap_mk a0 a1 (b0+c*2^a0) (b1+c*2^a1-k))
+| Nmap_c b0 b1 =>
+  Nsubge b1 k &&& (fun b2 =>
+  Some (Nmap_c b0 b2))
+end.
+
+Definition Nmap_divpow2 x k :=
+match x with
+| Nmap_mk a0 a1 b0 b1 =>
+  let pk:=2^k in
+  Ndiv b1 pk &&& (fun b1 => Some (Nmap_mk (a0+(k-a1)) (a1-k) b0 b1))
+| Nmap_c b0 b1 =>
+  Ndiv b1 (2^k) &&& (fun b1 => Some (Nmap_c b0 b1))
+end.
+
+Definition Nmap_mulpow2 x k :=
+match x with
+| Nmap_mk a0 a1 b0 b1 => Some (Nmap_mk a0 (a1+k) b0 (b1*2^k))
+| Nmap_c b0 b1 => Some (Nmap_c b0 (b1*2^k))
+end.
+
+Definition Nmap_to_c x k :=
+match x with
+| Nmap_mk a0 a1 b0 b1 =>
+  Nsubge k b1 &&& (fun k =>
+  Ndiv k (2^a1) &&& (fun k =>
+  Some (Nmap_c (2^a0*k+b0) (2^a1*k+b1))))
+| Nmap_c b0 b1 =>
+  if b1=?k then Some x else None
+end.
+
+Definition vN_to_c x k :=
+match x with
+| vN_v id mp => Nmap_to_c mp k &&& (fun mp => Some (vN_v id mp))
+| vN_c c => if c=?k then Some x else None
+end.
+
+Definition vN_subdivmulpow2 x m a0 a1 :=
+match x with
+| vN_v id mp =>
+  Nmap_sub mp m &&& (fun mp =>
+  Nmap_divpow2 mp a0 &&& (fun mp =>
+  Nmap_mulpow2 mp a1 &&& (fun mp =>
+  Some (vN_v id mp))))
+| vN_c c =>
+  Nsubge c m &&& (fun c =>
+  Ndiv c (2^a0) &&& (fun c =>
+  Some (vN_c (c*2^a1))))
+end.
+
+Definition vhead_c h n := vhead_mk h n (vN_c n).
+
+Lemma vN_is0'_spec n u:
+  vN_is0' n = Some u ->
+  vN_eval n 0.
+Proof.
+  unfold vN_is0'.
+  intros.
+  destruct n.
+  1: inverts H.
+  destruct (N.eqb_spec c 0).
+  2: inverts H.
+  subst.
+  ec.
+Qed.
+
+Lemma vN_is0_spec n u:
+  vN_is0 n = Some u ->
+  forall nv,
+  vN_eval n nv ->
+  nv=0.
+Proof.
+  unfold vN_is0.
+  intros.
+  destruct n.
+  1: {
+    destruct mp.
+    1: congruence.
+    destruct (N.eqb_spec b1 0).
+    2: inverts H.
+    subst.
+    inverts H0.
+    inverts H4.
+    ec.
+  }
+  destruct (N.eqb_spec c 0).
+  2: inverts H.
+  subst.
+  inverts H0.
+  ec.
+Qed.
+
+Definition vN_sub1 n n' :=
+vN_subdivmulpow2 n' 1 0 0 &&& (fun n' =>
+if n=?0 then vN_to_c n' 0 else Some n').
+
+Fixpoint segRLs_rec(hs:list vhead)(ws:list seg)(flag:bool)(T:nat):option((list vhead)*(list seg)) :=
+match T with
+| O => None
+| S T =>
+match ws with
+| [] => Some (hs,[])
+| w::ws =>
+match hs with
+| [] => Some ([],w::ws)
+| (vhead_mk h n n')::hs =>
+  (b2o flag &&& (fun _ =>
+  N_OS n &&& (fun _ =>
+  f2 w h &&& (fun '(a0,a1,h') =>
+  let pa0:=2^a0 in
+  let n1:=(n/pa0)*2^a1 in
+  let n2:=n mod pa0 in
+  vN_subdivmulpow2 n' n2 a0 a1 &&& (fun n' =>
+  segRLs_rec [vhead_mk h' n1 n'] ws true T &&& (fun '(hs',ws') =>
+  segRLs_rec ((vhead_c h n2)::hs) (w::ws') false T &&& (fun '(hs'0,ws'0) =>
+  Some (vheads_simpl hs' hs'0,ws'0)
+  ))))))) ||| (fun _ =>
+  match N_OS n with
+  | Some n =>
+    vN_sub1 n n' &&& (fun n' =>
+    f1 w h &&& (fun '(w',h') =>
+    segRLs_rec (vheads_simpl (map (fun h => vhead_c h 1) h') []) ws true T &&& (fun '(hs',ws') =>
+    segRLs_rec ((vhead_mk h n n')::hs) (w'++ws') flag T &&& (fun '(hs'0,ws'0) =>
+    Some (vheads_simpl hs' hs'0,ws'0)
+    ))))
+  | None =>
+    vN_to_c n' 0 &&& (fun n' =>
+    segRLs_rec hs (w::ws) true T &&& (fun '(hs',ws') =>
+    Some (vheads_simpl [vhead_mk h 0 n'] hs',ws')
+    ))
+  end)
+end
+end
+end.
+
+Fixpoint segRLs_rec' hs ws T :=
+match ws with
+| [] => Some (hs,[])
+| w::ws =>
+  segRLs_rec hs [w] true T &&& (fun '(hs',ws') =>
+  segRLs_rec' hs' ws T &&& (fun '(hs'0,ws'0) =>
+  Some (hs'0,ws'++ws'0)))
+end.
+
+Fixpoint sideRLs_rec hs ws w T :=
+match T with
+| O => None
+| S T =>
+  segRLs_rec' hs ws T &&& (fun '(hs,ws0) =>
+  match hs with
+  | [] => Some (ws0,w)
+  | vhead_mk h n n'::hs =>
+    match N_OS n with
+    | Some n =>
+      vN_sub1 n n' &&& (fun n' =>
+      f0 w h &&& (fun '(ws1,w') =>
+      sideRLs_rec (vhead_mk h n n'::hs) ws1 w' T &&& (fun '(ws',w') =>
+      Some (ws0++ws',w'))))
+    | None =>
+      vN_is0' n' &&& (fun _ =>
+      sideRLs_rec hs [] w T &&& (fun '(ws',w') =>
+      Some (ws0++ws',w')))
+    end
+  end)
+end.
+
+Lemma Nmap_sub_spec mp k mp':
+  Nmap_sub mp k = Some mp' ->
+  forall n n',
+  Nmap_apply mp' n n' ->
+  Nmap_apply mp n (n'+k).
+Proof.
+  unfold Nmap_sub.
+  intros.
+  destruct mp.
+  - inverts H.
+    inverts H0.
+    remember ((k-b1+(2^a1-1))/2^a1) as c.
+    applys_eq (Nmap_apply_mk a0 a1 b0 b1 (n0+c)); lia.
+  - des_if' H.
+    inverts H.
+    apply Nsubge_spec in E.
+    subst.
+    inverts H0.
+    ec.
+Qed.
+
+Lemma Nmap_divpow2_spec mp k mp':
+  Nmap_divpow2 mp k = Some mp' ->
+  forall n n',
+  Nmap_apply mp' n n' ->
+  Nmap_apply mp n (n'*2^k).
+Proof.
+  unfold Nmap_divpow2.
+  intros.
+  destruct mp.
+  - des_if H; inverts H.
+    apply Ndiv_spec in E.
+    subst b1.
+    inverts H0.
+    applys_eq (Nmap_apply_mk a0 a1 b0 (n0*2^k) (2^(k-a1)*n1)).
+    1: rewrite N.pow_add_r; lia.
+    rewrite N.mul_add_distr_r.
+    f_equal.
+    rewrite N.mul_shuffle0.
+    rewrite N.mul_assoc.
+    f_equal.
+    do 2 rewrite <-N.pow_add_r.
+    f_equal.
+    lia.
+  - des_if H; inverts H.
+    apply Ndiv_spec in E.
+    subst b1.
+    inverts H0.
+    ec.
+Qed.
+
+Lemma Nmap_mulpow2_spec mp k mp':
+  Nmap_mulpow2 mp k = Some mp' ->
+  forall n n',
+  Nmap_apply mp' n n' ->
+  exists n'0,
+  Nmap_apply mp n n'0 /\
+  n'=n'0*2^k.
+Proof.
+  unfold Nmap_mulpow2.
+  intros.
+  destruct mp.
+  - inverts H.
+    inverts H0.
+    eexists (2^a1*n0+b1); split.
+    2: rewrite N.pow_add_r; lia.
+    constructor.
+  - inverts H.
+    inverts H0.
+    eexists; split; ec.
+Qed.
+
+Lemma vN_subdivmulpow2_spec x m a0 a1 x':
+  vN_subdivmulpow2 x m a0 a1 = Some x' ->
+  forall x'v,
+  vN_eval x' x'v ->
+  exists xv,
+  vN_eval x xv /\
+  exists v,
+  xv = m+v*2^a0 /\
+  x'v = v*2^a1.
+Proof.
+  unfold vN_subdivmulpow2.
+  intros.
+  destruct x.
+  - do 3 des_if' H.
+    inverts H.
+    inverts H0.
+    eapply Nmap_mulpow2_spec in E1.
+    2: eauto 1.
+    destruct E1 as [n'0 [E1 E1a]].
+    subst x'v.
+    eapply Nmap_divpow2_spec in E0.
+    2: eauto 1.
+    eapply Nmap_sub_spec in E.
+    2: eauto 1.
+    eexists; split.
+    1: ec; eauto 1.
+    eexists n'0; lia.
+  - do 2 des_if' H.
+    inverts H.
+    apply Nsubge_spec in E.
+    apply Ndiv_spec in E0.
+    subst c n.
+    inverts H0.
+    eexists; split.
+    1: ec.
+    eexists n0; lia.
+Qed.
+
+Lemma Nmap_to_c_spec mp k mp':
+  Nmap_to_c mp k = Some mp' ->
+  forall n n',
+  Nmap_apply mp' n n' ->
+  Nmap_apply mp n k /\ k=n'.
+Proof.
+  unfold Nmap_to_c.
+  intros.
+  destruct mp.
+  - do 2 des_if' H.
+    inverts H.
+    apply Nsubge_spec in E.
+    apply Ndiv_spec in E0.
+    subst.
+    inverts H0.
+    rewrite (N.mul_comm n1).
+    ec; ec.
+  - destruct (N.eqb_spec b1 k); [subst|congruence].
+    inverts H.
+    inverts H0.
+    ec; ec.
+Qed.
+
+Lemma vN_to_c_spec x n x':
+  vN_to_c x n = Some x' ->
+  forall x'v,
+  vN_eval x' x'v ->
+  vN_eval x n /\ n=x'v.
+Proof.
+  unfold vN_to_c.
+  intros.
+  destruct x.
+  - des_if' H; inverts H.
+    inverts H0.
+    eapply Nmap_to_c_spec in E.
+    2: eauto 1.
+    destruct E as [Ea Eb].
+    subst.
+    ec; ec; trivial.
+  - destruct (N.eqb_spec c n); [subst|congruence].
+    inverts H.
+    inverts H0.
+    repeat ec.
+Qed.
+
+Lemma vN_sub1_spec n x x':
+  vN_sub1 n x = Some x' ->
+  forall x'v,
+  vN_eval x' x'v ->
+  vN_eval x (1+x'v).
+Proof.
+  unfold vN_sub1.
+  intros.
+  des_if' H.
+  destruct (N.eqb_spec n 0).
+  - inverts H.
+    subst.
+    eapply vN_to_c_spec in H2.
+    2: eauto 1.
+    destruct H2 as [H2 H2a]; subst.
+    eapply vN_subdivmulpow2_spec in E.
+    2: eauto 1.
+    destruct E as [xv [Ea [v0 [Eb Ec]]]].
+    subst.
+    applys_eq Ea; lia.
+  - inverts H.
+    eapply vN_subdivmulpow2_spec in E.
+    2: eauto 1.
+    destruct E as [xv [Ea [v [Eb Ec]]]].
+    subst.
+    eauto 1.
+Qed.
+
+Lemma Nmap_add_spec mp k:
+  let mp':=Nmap_add mp k in
+  forall n n',
+  Nmap_apply mp' n n' ->
+  exists n'0,
+  Nmap_apply mp n n'0 /\
+  n'=n'0+k.
+Proof.
+  unfold Nmap_add.
+  intros.
+  destruct mp.
+  - inverts H.
+    eexists (2^a1*n0+b1); split.
+    1: ec.
+    lia.
+  - inverts H.
+    eexists; split; ec.
+Qed.
+
+Lemma vN_add_spec a b c:
+  vN_add a b = Some c ->
+  forall cv,
+  vN_eval c cv ->
+  exists av bv,
+  vN_eval a av /\
+  vN_eval b bv /\
+  cv=av+bv.
+Proof.
+  unfold vN_add.
+  intros.
+  destruct a,b; inverts H.
+  - inverts H0.
+    apply Nmap_add_spec in H3.
+    destruct H3 as [n'0 [I1 I2]].
+    subst cv.
+    eex.
+    + ec; eauto 1.
+    + ec.
+  - inverts H0.
+    apply Nmap_add_spec in H3.
+    destruct H3 as [n'0 [I1 I2]].
+    subst cv.
+    eexists c1,n'0.
+    eex.
+    + ec.
+    + ec; eauto 1.
+    + lia.
+  - inverts H0.
+    eex; ec.
+Qed.
+
+Lemma vhead_add_spec a b c:
+  vhead_add a b = Some c ->
+  forall cv,
+  vhead_eval c cv ->
+  exists av bv,
+  vhead_eval a av /\
+  vhead_eval b bv /\
+  cv=av++bv.
+Proof.
+  unfold vhead_add.
+  intros.
+  destruct a,b.
+  des_if' H.
+  des_if' H.
+  inverts H.
+  destruct (eqb_spec h h0); inverts E; subst.
+  inverts H0.
+  eapply vN_add_spec in E0.
+  2: eauto 1.
+  destruct E0 as [av [bv [I1 [I2 I3]]]].
+  subst n'2.
+  eex.
+  1,2: eauto 1.
+  rewrite Nnat.N2Nat.inj_add,lpow_add.
+  reflexivity.
+Qed.
+
+Lemma vheads_simpl_spec ls ls0 lsv:
+  vheads_eval (vheads_simpl ls ls0) lsv ->
+  vheads_eval (ls++ls0) lsv.
+Proof.
+  gen ls0 lsv.
+  induction ls; cbn[vheads_simpl]; intros.
+  - apply H.
+  - destruct (vhead_is0' a) eqn:E'.
+    1:{
+      destruct a.
+      inverts E'.
+      eapply vN_is0'_spec in H1.
+      eapply IHls in H.
+      change lsv with ([]++lsv).
+      ec.
+      2: eauto 1.
+      eapply vhead_eval_mk in H1.
+      eauto 1.
+    }
+    destruct (vheads_simpl ls ls0) as [|h1 t1] eqn:E.
+    + epose proof (IHls _ _) as IHls.
+      rewrite E in IHls.
+      unshelve epose proof (IHls _) as IHls.
+      1: ec.
+      inverts H.
+      inverts H4.
+      ec; eauto 1.
+    + destruct (vhead_add a h1) eqn:E0.
+      * inverts H.
+        eapply vhead_add_spec in E0.
+        2: eauto 1.
+        destruct E0 as [av [bv [I1 [I2 I3]]]].
+        subst h'.
+        epose proof (IHls _ _) as IHls.
+        rewrite E in IHls.
+        unshelve epose proof (IHls _) as IHls.
+        1: ec; eauto 1.
+        rewrite <-app_assoc.
+        ec; eauto 1.
+      * inverts H.
+        epose proof (IHls _ _) as IHls.
+        rewrite E in IHls.
+        unshelve epose proof (IHls _) as IHls.
+        1: eauto 1.
+        ec; eauto 1.
+Qed.
+
+Lemma vheads_eval_split a b cv:
+  vheads_eval (a++b) cv ->
+  exists av bv,
+  vheads_eval a av /\
+  vheads_eval b bv /\
+  cv=av++bv.
+Proof.
+  gen b cv.
+  induction a; intros.
+  - eex.
+    1: ec.
+    1: eauto 1.
+    1: eauto 1.
+  - inverts H.
+    eapply IHa in H4.
+    destruct H4 as [av [bv [I1 [I2 I3]]]].
+    subst.
+    eexists _,_; split.
+    1: ec; eauto 1.
+    split.
+    1: eauto 1.
+    apply app_assoc.
+Qed.
+
+Lemma vheads_c_spec h hv:
+  vheads_eval (map (fun h : head => vhead_c h 1) h) hv ->
+  hv = h.
+Proof.
+  gen hv.
+  induction h; intros.
+  - inverts H; trivial.
+  - inverts H.
+    apply IHh in H4.
+    inverts H2.
+    inverts H5.
+    subst; trivial.
+Qed.
+
+Local Opaque vheads_simpl.
+
+Lemma segRLs_rec_spec hs ws flag T hs' ws':
+  segRLs_rec hs ws flag T = Some (hs',ws') ->
+  forall hs'v,
+  vheads_eval hs' hs'v ->
+  exists hsv,
+  vheads_eval hs hsv /\
+  segRLs tm hsv hs'v (concat ws) (concat ws').
+Proof.
+  gen hs ws flag hs' ws'.
+  induction T; intros.
+  1: inverts H.
+  cbn[segRLs_rec] in H.
+  destruct ws as [|w ws].
+  { inverts H.
+    eexists; split.
+    1: apply H0.
+    apply segRLs_nil. }
+  destruct hs as [|[h n n'] hs].
+  { inverts H.
+    inverts H0.
+    eexists; split; constructor. }
+  des_if H.
+  {
+    inverts H.
+    do 2 des_if' E.
+    clear E1.
+    des_if' E.
+    destruct p as [[a0 a1] h'].
+    do 2 des_if' E.
+    destruct p as [hs'0 ws'0].
+    des_if' E.
+    destruct p as [hs'1 ws'1].
+    inverts E.
+    eapply f2_spec in E1.
+    eapply vheads_simpl_spec in H0.
+    eapply vheads_eval_split in H0.
+    destruct H0 as [av [bv [I1 [I2 I3]]]].
+    subst.
+    eapply IHT in E4.
+    2: eauto 1.
+    destruct E4 as [hs'1v [E4a E4b]].
+    eapply IHT in E3.
+    2: eauto 1.
+    destruct E3 as [hsv [E3a E3b]].
+    inverts E4a.
+    inverts E3a.
+    inverts H5.
+    inverts H2.
+    eapply vN_subdivmulpow2_spec in E2.
+    2: eauto 1.
+    destruct E2 as [xv [E2a [v0 [E2b E2c]]]].
+    subst.
+    eexists; split.
+    - ec.
+      2: eauto 1.
+      ec; eauto 1.
+    - rewrite N.add_comm.
+      rewrite Nnat.N2Nat.inj_add,lpow_add,<-app_assoc.
+      rewrite app_nil_r in E3b.
+      eapply segRLs_trans.
+      + cbn[concat].
+        eapply segRLs_concat.
+        2: eauto 1.
+        do 2 rewrite Nnat.N2Nat.inj_mul.
+        do 2 rewrite lpow_mul.
+        eapply segRLs_wall''.
+        eauto 1.
+      + inverts H1.
+        inverts H5.
+        eauto 1.
+  }
+  clear E.
+  {
+    cbn in H.
+    epose proof (N_OS_spec n) as E.
+    destruct (N_OS n) as [n0|]; subst n.
+    { 
+      do 2 des_if' H.
+      destruct p as [w' h'].
+      des_if' H.
+      destruct p as [hs'0 ws'0].
+      des_if' H.
+      destruct p as [hs'1 ws'1].
+      inverts H.
+      eapply vheads_simpl_spec in H0.
+      eapply vheads_eval_split in H0.
+      destruct H0 as [av [bv [I1 [I2 I3]]]].
+      subst.
+      eapply IHT in E2.
+      2: eauto 1.
+      destruct E2 as [hsv [E2a E2b]].
+      eapply IHT in E1.
+      2: eauto 1.
+      destruct E1 as [hsv0 [E1a E1b]].
+      eapply f1_spec in E0.
+      inverts E2a.
+      inverts H1.
+      eapply vN_sub1_spec in E.
+      2: eauto 1.
+      eapply vheads_simpl_spec in E1a.
+      rewrite app_nil_r in E1a.
+      apply vheads_c_spec in E1a.
+      subst hsv0.
+      eexists; split.
+      - ec.
+        2: eauto 1.
+        ec; eauto 1.
+      - rewrite Nnat.N2Nat.inj_add,lpow_add,<-app_assoc.
+        eapply segRLs_trans.
+        + cbn[concat].
+          eapply segRLs_concat; eauto 1.
+        + rewrite concat_app in E2b.
+          eauto 1. }
+    {
+      des_if' H.
+      des_if' H.
+      destruct p as [hs'0 ws'0].
+      inverts H.
+      eapply vheads_simpl_spec in H0.
+      inverts H0.
+      inverts H2.
+      eapply IHT in E0.
+      2: eauto 1.
+      destruct E0 as [hsv [I1 I2]].
+      eapply vN_to_c_spec in E.
+      2: eauto 1.
+      destruct E as [E Ea]; subst.
+      eexists; split.
+      - ec.
+        2: eauto 1.
+        ec; eauto 1.
+      - eauto 1.
+    }
+  }
+Qed.
+
+Lemma segRLs_rec'_spec hs ws T hs' ws':
+  segRLs_rec' hs ws T = Some (hs',ws') ->
+  forall hs'v,
+  vheads_eval hs' hs'v ->
+  exists hsv,
+  vheads_eval hs hsv /\
+  segRLs tm hsv hs'v (concat ws) (concat ws').
+Proof.
+  gen hs T hs' ws'.
+  induction ws; intros.
+  - inverts H.
+    eexists; split.
+    1: apply H0.
+    apply segRLs_nil.
+  - cbn[segRLs_rec'] in H.
+    des_if' H.
+    destruct p as [hs'0 ws'0].
+    des_if' H.
+    destruct p as [hs'1 ws'1].
+    inverts H.
+    eapply IHws in E0.
+    2: eauto 1.
+    destruct E0 as [hsv [E0a E0b]].
+    eapply segRLs_rec_spec in E.
+    2: eauto 1.
+    destruct E as [hsv0 [Ea Eb]].
+    eexists; split.
+    + eauto 1.
+    + cbn[concat] in *.
+      rewrite app_nil_r in Eb.
+      rewrite concat_app.
+      eapply segRLs_concat; eauto 1.
+Qed.
+
+Lemma sideRLs_rec_spec hs ws w T ws':
+  sideRLs_rec hs ws w T = Some ws' ->
+  exists hs',
+  vheads_eval hs hs' /\
+  sideRLs tm hs' (to_side (ws,w)) (to_side ws').
+Proof.
+  gen hs ws w ws'.
+  induction T; intros.
+  1: inverts H.
+  cbn[sideRLs_rec] in H.
+  des_if' H.
+  destruct p as [hs0 ws1].
+  cbn in H.
+  destruct hs0 as [|h hs0].
+  - inverts H.
+    eapply segRLs_rec'_spec in E.
+    2: ec.
+    destruct E as [hsv [Ea Eb]].
+    unfold to_side.
+    eex.
+    1: eauto 1.
+    eapply segRLs_sideRLs_concat.
+    1: eauto 1.
+    ec.
+  - destruct h.
+    pose proof (N_OS_spec n) as E0.
+    destruct (N_OS n); subst n.
+    + des_if' H.
+      des_if' H.
+      destruct p as [ws2 w'].
+      des_if' H.
+      destruct p as [ws'0 w'0].
+      inverts H.
+      eapply IHT in E2.
+      destruct E2 as [hs' [E2a E2b]].
+      eapply f0_spec in E1.
+      inverts E2a.
+      inverts H1.
+      eapply vN_sub1_spec in E0.
+      2: eauto 1.
+      eapply segRLs_rec'_spec in E.
+      2: ec.
+      3: eauto 1.
+      2: ec; eauto 1.
+      destruct E as [hsv [Ea Eb]].
+      eex.
+      1: eauto 1.
+      unfold to_side.
+      rewrite concat_app,Str_app_assoc.
+      eapply segRLs_sideRLs_concat.
+      1: eauto 1.
+      rewrite Nnat.N2Nat.inj_add,lpow_add,<-app_assoc.
+      eapply sideRLs_trans; eauto 1.
+    + des_if' H.
+      des_if' H.
+      destruct p as [ws'0 w'].
+      inverts H.
+      eapply IHT in E1.
+      destruct E1 as [hs' [E1a E1b]].
+      eapply vN_is0'_spec in E0.
+      eapply segRLs_rec'_spec in E.
+      2: ec.
+      3: eauto 1.
+      2: ec; eauto 1.
+      destruct E as [hsv [Ea Eb]].
+      eex.
+      1: eauto 1.
+      unfold to_side.
+      rewrite concat_app,Str_app_assoc.
+      eapply segRLs_sideRLs_concat; eauto 1.
+Qed.
+
+End vhead_sec.
+
+Fixpoint lcp(ls ls0:list seg):list seg :=
+match ls,ls0 with
+| h::t,h0::t0 => if eqb h h0 then h::lcp t t0 else []
+| _,_ => []
+end.
+
+Fixpoint skip(ls ls0:list seg):option (list seg) :=
+match ls,ls0 with
+| h::t,h0::t0 => if eqb h h0 then skip t t0 else None
+| _,[] => Some ls
+| _,_ => None
+end.
+
+Fixpoint interpolate(ls ls0 ls1:list seg)(T:nat):option (list (list seg+list seg)) :=
+match T with
+| O => None
+| S T =>
+  if (eqb ls [] && eqb ls0 [] && eqb ls1 []) then Some [] else
+  let ls0' := lcp ls0 ls1 in
+  let ls' := lcp ls ls0' in
+  match ls' with
+  | [] =>
+    skip ls0 ls0' &&& (fun ls0 =>
+    skip ls1 ls0' &&& (fun ls1 =>
+    skip ls1 ls0' &&& (fun ls1 =>
+    interpolate ls ls0 ls1 T &&& (fun res =>
+    Some (inr ls0' :: res)))))
+  | _ =>
+    skip ls ls' &&& (fun ls =>
+    skip ls0 ls' &&& (fun ls0 =>
+    skip ls1 ls' &&& (fun ls1 =>
+    interpolate ls ls0 ls1 T &&& (fun res =>
+    (match res with
+    | inr ls'0 :: res =>
+      let n2:=length ls'0 in
+      let n1:=length ls' in
+      b2o (eqb ls'0 (skipn (n1-n2) ls')) &&& (fun _ =>
+      let ls' := firstn (n1-n2) ls' in
+      Some (inl ls' :: inr ls'0 :: inl ls'0 :: res))
+    | _ => None
+    end ||| (fun _ => Some (inl ls' :: res))))
+    )))
+  end
+end.
+
+Definition interpolate'(x0 x1 x2:list seg * seg) T :=
+match x0,x1,x2 with
+| (ws0,w0),(ws1,w1),(ws2,w2) =>
+  b2o (eqb w0 w1 && eqb w0 w2) &&& (fun _ =>
+  interpolate ws0 ws1 ws2 T &&& (fun ws =>
+  Some (ws,w0)))
+end.
+
+Fixpoint vheads_v hs id (f:N->bool) :=
+match hs with
+| vhead_mk h n _::hs =>
+  vhead_mk h n (if f id then vN_c n else vN_v id (Nmap_mk 0 0 0 0))::vheads_v hs (id+1) f
+| [] => []
+end.
+
+Fixpoint get_del_vars hs :=
+match hs with
+| vhead_mk h 0 (vN_v id _)::hs =>
+  fun x => if x =? id then true else get_del_vars hs x
+| _::hs => get_del_vars hs
+| [] => fun _ => false
+end.
+
+
+Ltac rw_pa := repeat rewrite N.pow_add_r in *.
+
+Lemma Nmap_applys_inc a0 a1 b0 b1 n k:
+  a1<>0 ->
+  Nmap_applys (Nmap_mk a0 (a0+a1) b0 (b0+2^a0*b1)) (2^a0*n+b0) (2^a0*2^(a1*k)*n+(b0+(2^(a1*k)-1)/(2^a1-1)*(2^a0*b1))) k.
+Proof.
+  gen a0 a1 b0 b1 n.
+  induction k using N.peano_ind; intros.
+  - applys_eq Nmap_applys_O.
+    repeat rewrite N.mul_0_r.
+    lia.
+  - replace (N.succ k) with (1+k) by lia.
+    eapply Nmap_applys_S.
+    1: ec.
+    replace (a1*(1+k)) with (a1+a1*k) by lia.
+    rw_pa.
+    applys_eq (IHk a0 a1 b0 b1 (2^a1*n+b1)).
+    1,3: lia.
+    remember (2^(a1*k)) as v2.
+    remember (2^a1-1) as v1.
+    assert (v1<>0). {
+      replace a1 with (1+(a1-1)) in * by lia.
+      rw_pa; lia.
+    }
+    replace (2^a1) with (v1+1) in * by lia.
+    replace ((v1+1)*v2-1) with (v2-1+v2*v1) by lia.
+    rewrite N.div_add by lia.
+    lia.
+Qed.
+
+Lemma Nmap_applys_S' mp n0 n1 n2 k:
+  Nmap_applys mp n0 n1 k ->
+  Nmap_apply mp n1 n2 ->
+  Nmap_applys mp n0 n2 (1+k).
+Proof.
+  intro H.
+  induction H; intros.
+  - ec.
+    1: eauto 1.
+    ec.
+  - ec; eauto 2.
+Qed.
+
+Lemma Nmap_apply_rev a0 a1 b0 b1 n0 n1:
+  Nmap_apply (Nmap_mk a0 a1 b0 b1) n0 n1 ->
+  Nmap_apply (Nmap_mk a1 a0 b1 b0) n1 n0.
+Proof.
+  intros.
+  inverts H.
+  ec.
+Qed.
+
+Local Opaque N.add.
+
+Lemma Nmap_applys_rev a0 a1 b0 b1 n0 n1 k:
+  Nmap_applys (Nmap_mk a0 a1 b0 b1) n0 n1 k ->
+  Nmap_applys (Nmap_mk a1 a0 b1 b0) n1 n0 k.
+Proof.
+  gen a0 a1 b0 b1 n0 n1.
+  induction k using N.peano_ind; intros.
+  - inverts H; [ec|lia].
+  - replace (N.succ k) with (1+k) in * by lia.
+    inverts H; [lia|].
+    replace k0 with k in * by lia.
+    eapply Nmap_applys_S'.
+    + eauto 2.
+    + eapply Nmap_apply_rev; eauto 1.
+Qed.
+
+Lemma Nmap_applys_dec a0 a1 b0 b1 n k:
+  a1<>0 ->
+  Nmap_applys (Nmap_mk (a0+a1) a0 (b0+2^a0*b1) b0) (2^a0*2^(a1*k)*n+(b0+(2^(a1*k)-1)/(2^a1-1)*(2^a0*b1))) (2^a0*n+b0) k.
+Proof.
+  intros.
+  apply Nmap_applys_rev.
+  apply Nmap_applys_inc; auto 1.
+Qed.
+
+Inductive N' :=
+| N'_mk(a b c d:N)
+| N'_c(a:N).
+
+Definition toN(n:N)(x:N'):N :=
+match x with
+| N'_mk a b c d => ((2^(n*a)-1)*b+c)/d
+| N'_c a => a
+end.
+
+Definition N'_eq_c x k :=
+match x with
+| N'_c c => b2o (c =? k)
+| _ => None
+end.
+
+Ltac des_N_op :=
+repeat
+match goal with
+| [H: b2o (?a =? ?b) = Some _ |- _] =>
+  destruct (N.eqb_spec a b); inverts H; subst
+| [H: b2o (negb (?a =? ?b)) = Some _ |- _] =>
+  destruct (N.eqb_spec a b); inverts H
+| [H: b2o (eqb ?a ?b) = Some _ |- _] =>
+  destruct (eqb_spec a b); inverts H; subst
+| [H: Nsubge ?a ?b = Some _ |- _] =>
+  apply Nsubge_spec in H; subst
+| [H: Ndiv ?a ?b = Some _ |- _] =>
+  apply Ndiv_spec in H; subst
+end.
+
+Lemma N'_eq_c_spec x k u n:
+  N'_eq_c x k = Some u ->
+  toN n x = k.
+Proof.
+  unfold N'_eq_c.
+  intros.
+  destruct x.
+  1: inverts H.
+  des_N_op.
+  trivial.
+Qed.
+
+Definition N'_Nmap_apply mp x :=
+match mp with
+| Nmap_mk a0 a1 b0 b1 =>
+  match x with
+  | N'_c c =>
+    Nsubge c b0 &&& (fun c =>
+    Ndiv c (2^a0) &&& (fun c =>
+    Some (N'_c (c*2^a1+b1))))
+  | N'_mk a b c d =>
+    Nsubge c (b0*d) &&& (fun c =>
+    Ndiv b (2^a0*d) &&& (fun b =>
+    Ndiv c (2^a0*d) &&& (fun c =>
+    b2o (negb (d=?0)) &&& (fun _ =>
+    Some (N'_mk a (b*2^a1*d) ((c*2^a1+b1)*d) d)))))
+  end
+| Nmap_c b0 b1 =>
+  N'_eq_c x b0 &&& (fun _ =>
+  Some (N'_c b1))
+end.
+
+Lemma N'_Nmap_apply_spec mp x x' n:
+  N'_Nmap_apply mp x = Some x' ->
+  Nmap_apply mp (toN n x) (toN n x').
+Proof.
+  unfold N'_Nmap_apply.
+  intros.
+  destruct mp.
+  - destruct x.
+    + do 4 des_if' H.
+      inverts H.
+      des_N_op.
+      unfold toN.
+      repeat rewrite N.mul_assoc.
+      repeat rewrite <-N.mul_add_distr_r.
+      repeat rewrite N.div_mul by auto 1.
+      applys_eq (Nmap_apply_mk a0 a1 b0 b1 ((2^(n*a)-1)*n1+n2)); lia.
+    + do 2 des_if' H.
+      inverts H.
+      des_N_op.
+      unfold toN.
+      applys_eq (Nmap_apply_mk a0 a1 b0 b1 n1); lia.
+  - des_if' H.
+    inverts H.
+    eapply N'_eq_c_spec in E.
+    rewrite E.
+    ec.
+Qed.
+
+Definition N'_Nmap_applys_inc_0(a0 a1 b0 b1:N)(x:N'):option N' :=
+match x with
+| N'_c n =>
+  b2o (negb (a1=?0)) &&& (fun _ =>
+  Nsubge n b0 &&& (fun n =>
+  Ndiv n (2^a0) &&& (fun n =>
+  Some (N'_mk a1 (2^a0*(b1+n*(2^a1-1))) ((2^a0*n+b0)*(2^a1-1)) (2^a1-1)))))
+| _ => None
+end.
+
+Definition N'_simpl_d x :=
+match x with
+| N'_mk a b c d =>
+  let g:=N.gcd d (N.gcd b c) in
+  b2o (negb (g=?0)) &&& (fun _ =>
+  Ndiv b g &&& (fun b =>
+  Ndiv c g &&& (fun c =>
+  Ndiv d g &&& (fun d =>
+  Some (N'_mk a b c d)))))
+| _ => None
+end.
+
+Lemma N'_simpl_d_spec x x' n:
+  N'_simpl_d x = Some x' ->
+  toN n x = toN n x'.
+Proof.
+  unfold N'_simpl_d.
+  intros.
+  destruct x.
+  2: inverts H.
+  do 4 des_if' H.
+  inverts H.
+  des_N_op.
+  remember (N.gcd d (N.gcd b c)) as v1.
+  clear Heqv1.
+  subst.
+  unfold toN.
+  rewrite N.mul_assoc.
+  rewrite <-N.mul_add_distr_r.
+  rewrite N.Div0.div_mul_cancel_r; trivial.
+Qed.
+
+Definition N'_Nmap_applys_inc(a0 a1 b0 b1:N)(x:N'):option N' :=
+N'_Nmap_applys_inc_0 a0 a1 b0 b1 x &&& (fun x =>
+N'_simpl_d x).
+
+Lemma geosum_div a n:
+  (2^(n*a)-1) mod (2^a-1) = 0.
+Proof.
+  intros.
+  induction n using N.peano_ind.
+  - rewrite N.mul_0_l; trivial.
+  - rewrite N.mul_succ_l.
+    rw_pa.
+    remember (2^(n*a)-1) as v1. 
+    replace (2^(n*a)) with (v1+1) in * by lia.
+    remember (2^(a)-1) as v2. 
+    replace (2^(a)) with (v2+1) in * by lia.
+    replace ((v1+1)*(v2+1)-1) with (v1+(v1+1)*v2) by lia.
+    rewrite N.Div0.mod_add; trivial.
+Qed.
+
+Lemma N'_Nmap_applys_inc_0_spec a0 a1 b0 b1 x x' n:
+  N'_Nmap_applys_inc_0 a0 a1 b0 b1 x = Some x' ->
+  Nmap_applys (Nmap_mk a0 (a0+a1) b0 (b0+2^a0*b1)) (toN n x) (toN n x') n.
+Proof.
+  unfold N'_Nmap_applys_inc_0.
+  intros.
+  destruct x.
+  1: inverts H.
+  do 3 des_if' H.
+  inverts H.
+  des_N_op.
+  unfold toN.
+  pose proof (geosum_div a1 n) as I1.
+  applys_eq (Nmap_applys_inc a0 a1 b0 b1 n1 n).
+  1,3: lia.
+  remember (2^a1-1) as v1.
+  assert (v1<>0) by (pose proof (N.pow_le_mono_r 2 1 a1); lia).
+  replace (2^a1) with (v1+1) in * by lia.
+  rewrite (N.mul_comm a1 n).
+  remember (2^(n*a1)-1) as v2.
+  replace (2^(n*a1)) with (v2+1) in * by lia.
+  repeat rewrite N.mul_assoc.
+  repeat rewrite N.add_assoc.
+  rewrite N.div_add by lia.
+  rewrite <-N.mul_assoc,N.mul_comm.
+  rewrite N.Lcm0.divide_div_mul_exact.
+  2: apply N.Lcm0.mod_divide,I1.
+  pose proof (N.div_mod v2 v1) as I2.
+  rewrite I1 in I2.
+  lia.
+Qed.
+
+Lemma N'_Nmap_applys_inc_spec a0 a1 b0 b1 x x' n:
+  N'_Nmap_applys_inc a0 a1 b0 b1 x = Some x' ->
+  Nmap_applys (Nmap_mk a0 (a0+a1) b0 (b0+2^a0*b1)) (toN n x) (toN n x') n.
+Proof.
+  unfold N'_Nmap_applys_inc.
+  intros.
+  des_if' H.
+  inverts H.
+  eapply N'_Nmap_applys_inc_0_spec in E.
+  eapply N'_simpl_d_spec in H1.
+  rewrite H1 in E.
+  apply E.
+Qed.
+
+Definition N'_set_d x k :=
+match x with
+| N'_mk a b c d =>
+  Ndiv k d &&& (fun k =>
+  b2o (negb (k =? 0)) &&& (fun _ =>
+  Some (N'_mk a (b*k) (c*k) (d*k))))
+| _ => None
+end.
+
+Lemma N'_set_d_spec x k x' n:
+  N'_set_d x k = Some x' ->
+  toN n x = toN n x'.
+Proof.
+  unfold N'_set_d.
+  intros.
+  destruct x.
+  2: inverts H.
+  do 2 des_if' H.
+  inverts H.
+  des_N_op.
+  unfold toN.
+  rewrite N.mul_assoc.
+  rewrite <-N.mul_add_distr_r.
+  rewrite N.Div0.div_mul_cancel_r; trivial.
+Qed.
+
+Definition N'_Nmap_applys_dec(a0 a1 b0 b1:N)(x:N'):option N' :=
+N'_set_d x (2^a1-1) &&& (fun x =>
+match x with
+| N'_mk a b c d =>
+  b2o (negb (a1=?0)) &&& (fun _ =>
+  b2o (a=?a1) &&& (fun _ =>
+  b2o (d =? 2^a1-1) &&& (fun _ =>
+  Nsubge b (2^a0*b1) &&& (fun b =>
+  Ndiv b (2^a0*d) &&& (fun n =>
+  b2o (c =? ((2^a0*n+b0)*d)) &&& (fun _ =>
+  Some (N'_c (n*2^a0+b0))))))))
+| _ => None
+end).
+
+Lemma N'_Nmap_applys_dec_spec a0 a1 b0 b1 x x' n:
+  N'_Nmap_applys_dec a0 a1 b0 b1 x = Some x' ->
+  Nmap_applys (Nmap_mk (a0+a1) a0 (b0+2^a0*b1) b0) (toN n x) (toN n x') n.
+Proof.
+  unfold N'_Nmap_applys_dec.
+  intros.
+  destruct x.
+  2: inverts H.
+  des_if' H.
+  cbn in H.
+  destruct n0.
+  2: inverts H.
+  do 6 des_if' H.
+  inverts H.
+  des_N_op.
+  eapply N'_set_d_spec in E.
+  rewrite E; clear E.
+  unfold toN.
+  pose proof (geosum_div a1 n) as I1.
+  applys_eq (Nmap_applys_dec a0 a1 b0 b1 n1 n).
+  2,3: lia.
+  remember (2^a1-1) as v1.
+  assert (v1<>0) by (pose proof (N.pow_le_mono_r 2 1 a1); lia).
+  replace (2^a1) with (v1+1) in * by lia.
+  rewrite (N.mul_comm a1 n).
+  remember (2^(n*a1)-1) as v2.
+  replace (2^(n*a1)) with (v2+1) in * by lia.
+  repeat rewrite N.mul_assoc.
+  repeat rewrite N.add_assoc.
+  rewrite N.div_add by lia.
+  rewrite <-N.mul_assoc,N.mul_comm.
+  rewrite N.Lcm0.divide_div_mul_exact.
+  2: apply N.Lcm0.mod_divide,I1.
+  pose proof (N.div_mod v2 v1) as I2.
+  rewrite I1 in I2.
+  lia.
+Qed.
+
+Definition N'_Nmap_applys_id(a0 b0:N)(x:N'):option N' :=
+N'_Nmap_apply (Nmap_mk a0 a0 b0 b0) x.
+
+Definition N'_Nmap_applys_id_c(b0:N)(x:N'):option N' :=
+N'_Nmap_apply (Nmap_c b0 b0) x.
+
+Definition N'_Nmap_applys mp x :=
+match mp with
+| Nmap_mk a0 a1 b0 b1 =>
+  (b2o (a0=?a1) &&& (fun _ =>
+  b2o (b0=?b1) &&& (fun _ =>
+  N'_Nmap_applys_id a0 b0 x))) ||| (fun _ =>
+  (Nsubge a1 a0 &&& (fun a1 =>
+  Nsubge b1 b0 &&& (fun b1 =>
+  Ndiv b1 (2^a0) &&& (fun b1 =>
+  N'_Nmap_applys_inc a0 a1 b0 b1 x)))) ||| (fun _ =>
+  (Nsubge a0 a1 &&& (fun a0 =>
+  Nsubge b0 b1 &&& (fun b0 =>
+  Ndiv b0 (2^a1) &&& (fun b0 =>
+  N'_Nmap_applys_dec a1 a0 b1 b0 x))))))
+| Nmap_c b0 b1 =>
+  b2o (b0=?b1) &&& (fun _ =>
+  N'_Nmap_applys_id_c b0 x)
+end.
+
+Lemma Nmap_applys_id a0 b0 x x' n:
+  Nmap_apply (Nmap_mk a0 a0 b0 b0) x x' ->
+  Nmap_applys (Nmap_mk a0 a0 b0 b0) x x' n.
+Proof.
+  intros.
+  inverts H.
+  induction n using N.peano_ind.
+  1: ec.
+  replace (N.succ n) with (1+n) by lia.
+  ec.
+  2: eauto 1.
+  ec.
+Qed.
+
+Lemma N'_Nmap_applys_id_spec a0 b0 x x' n:
+  N'_Nmap_applys_id a0 b0 x = Some x' ->
+  Nmap_applys (Nmap_mk a0 a0 b0 b0) (toN n x) (toN n x') n.
+Proof.
+  unfold N'_Nmap_applys_id.
+  intros.
+  eapply N'_Nmap_apply_spec in H.
+  eapply Nmap_applys_id in H.
+  apply H.
+Qed.
+
+Lemma Nmap_applys_id_c b0 x x' n:
+  Nmap_apply (Nmap_c b0 b0) x x' ->
+  Nmap_applys (Nmap_c b0 b0) x x' n.
+Proof.
+  intros H.
+  inverts H.
+  induction n using N.peano_ind.
+  1: ec.
+  replace (N.succ n) with (1+n) by lia.
+  ec.
+  2: eauto 1.
+  ec.
+Qed.
+
+Lemma N'_Nmap_applys_id_c_spec b0 x x' n:
+  N'_Nmap_applys_id_c b0 x = Some x' ->
+  Nmap_applys (Nmap_c b0 b0) (toN n x) (toN n x') n.
+Proof.
+  unfold N'_Nmap_applys_id_c.
+  intros.
+  eapply N'_Nmap_apply_spec in H.
+  eapply Nmap_applys_id_c in H.
+  apply H.
+Qed.
+
+Lemma N'_Nmap_applys_spec mp x x' n:
+  N'_Nmap_applys mp x = Some x' ->
+  Nmap_applys mp (toN n x) (toN n x') n.
+Proof.
+  unfold N'_Nmap_applys.
+  intros.
+  destruct mp.
+  2:{
+    des_if' H.
+    inverts H.
+    des_N_op.
+    eapply N'_Nmap_applys_id_c_spec in H1.
+    apply H1.
+  }
+  des_if' H.
+  {
+    inverts H.
+    do 2 des_if' E.
+    inverts E.
+    des_N_op.
+    eapply N'_Nmap_applys_id_spec in H0.
+    apply H0.
+  }
+  clear E.
+  rename H1 into H.
+  des_if' H.
+  {
+    inverts H.
+    do 3 des_if' E.
+    inverts E.
+    des_N_op.
+    eapply N'_Nmap_applys_inc_spec in H0.
+    applys_eq H0; flia.
+  }
+  {
+    do 3 des_if' H1.
+    inverts H1.
+    des_N_op.
+    eapply N'_Nmap_applys_dec_spec in H0.
+    applys_eq H0; flia.
+  }
+Qed.
+
+Inductive N'_head :=
+| N'_head_mk(h0:head)(n:N').
+
+Definition Nmap_is_id mp :=
+match mp with
+| Nmap_mk 0 0 0 0 => Some tt
+| _ => None
+end.
+
+Fixpoint N'_match_vheads hs (hs':list (N'_head)) :=
+match hs,hs' with
+| vhead_mk h n n'::hs,(N'_head_mk h'0 h')::hs' =>
+  b2o (eqb h h'0) &&& (fun _ =>
+  N'_match_vheads hs hs' &&& (fun f =>
+  match n' with
+  | vN_v id mp =>
+    Nmap_is_id mp &&& (fun _ =>
+    Some (fun x => if x=?id then Some h' else f x))
+  | vN_c c =>
+    N'_eq_c h' c &&& (fun _ =>
+    Some f)
+  end))
+| [],[] => Some (fun _ => None)
+| _,_ => None
+end.
+
+Definition N'_eqb x x0 :=
+match x,x0 with
+| N'_mk a b c d,N'_mk a0 b0 c0 d0 => eqb a a0 && eqb b b0 && eqb c c0 && eqb d d0
+| N'_c c,N'_c c0 => eqb c c0
+| _,_ => false
+end.
+
+Instance N'_Eqb: Eqb N'.
+Proof with solve_Bool_reflect.
+  apply Build_Eqb with (eqb:=N'_eqb).
+  intros.
+  unfold N'_eqb.
+  destruct x,y...
+  - destruct (eqb_spec a a0)...
+    destruct (eqb_spec b b0)...
+    destruct (eqb_spec c c1)...
+    destruct (eqb_spec d d0)...
+  - destruct (eqb_spec a a0)...
+Defined.
+
+Fixpoint N'_matched_vheads hs (hs':list (N'_head)) f {struct hs} :=
+match hs,hs' with
+| vhead_mk h n n'::hs,(N'_head_mk h'0 h')::hs' =>
+  b2o (eqb h h'0) &&& (fun _ =>
+  N'_matched_vheads hs hs' f &&& (fun _ =>
+  match n' with
+  | vN_v id mp =>
+    Nmap_is_id mp &&& (fun _ =>
+    f id &&& (fun x => b2o (eqb x h')))
+  | vN_c c =>
+    N'_eq_c h' c
+  end))
+| [],[] => Some tt 
+| _,_ => None
+end.
+
+Fixpoint N'_apply_vheads hs f :=
+match hs with
+| vhead_mk h n n'::hs =>
+  N'_apply_vheads hs f &&& (fun res =>
+  match n' with
+  | vN_v id mp =>
+    f id &&& (fun x =>
+    N'_Nmap_apply mp x &&& (fun x =>
+    Some ((N'_head_mk h x)::res)))
+  | vN_c c =>
+    Some ((N'_head_mk h (N'_c c))::res)
+  end)
+| [] => Some []
+end.
+
+Fixpoint N'_applys_vheads hs f :=
+match hs with
+| vhead_mk h n n'::hs =>
+  N'_applys_vheads hs f &&& (fun res =>
+  match n' with
+  | vN_v id mp =>
+    f id &&& (fun x =>
+    N'_Nmap_applys mp x &&& (fun x =>
+    Some ((N'_head_mk h x)::res)))
+  | vN_c c =>
+    Some ((N'_head_mk h (N'_c c))::res)
+  end)
+| [] => Some []
+end.
+
+Fixpoint hs_match_rec hs hs' id0 :=
+match hs,hs' with
+| vhead_mk h n (vN_c c)::hs,vhead_mk h' n' (vN_c c')::hs' =>
+  b2o (eqb h h') &&& (fun _ =>
+  b2o (eqb c c') &&& (fun _ =>
+  hs_match_rec hs hs' id0))
+| vhead_mk h n (vN_v id mp)::hs,vhead_mk h' n' (vN_v id' mp')::hs' =>
+  b2o (eqb h h') &&& (fun _ =>
+  b2o (eqb id id') &&& (fun _ =>
+  b2o (id0 <=? id) &&& (fun _ =>
+  Nmap_is_id mp &&& (fun _ =>
+  hs_match_rec hs hs' (1+id)))))
+| [],[] => Some tt
+| _,_ => None
+end.
+
+Fixpoint segRLs_rec_v hsN' hs ws T :=
+let hs:=vheads_v hs 0 (fun _=>false) in
+match ws with
+| [] => Some (hsN',hs,[])
+| inl ws::ws0 =>
+  segRLs_rec' hs ws T &&& (fun '(hs',ws') =>
+  let hs:=vheads_v hs 0 (get_del_vars hs') in
+  segRLs_rec' hs ws T &&& (fun '(hs',ws') =>
+  N'_match_vheads hs hsN' &&& (fun f =>
+  N'_matched_vheads hs hsN' f &&& (fun _ =>
+  N'_apply_vheads hs' f &&& (fun hsN' =>
+  segRLs_rec_v hsN' hs' ws0 T &&& (fun '(res0,res) =>
+  Some (res0,inl ws'::res)))))))
+| inr ws::ws0 =>
+  segRLs_rec' hs ws T &&& (fun '(hs',ws') =>
+  let hs:=vheads_v hs 0 (get_del_vars hs') in
+  segRLs_rec' hs ws T &&& (fun '(hs',ws') =>
+  N'_match_vheads hs hsN' &&& (fun f =>
+  N'_matched_vheads hs hsN' f &&& (fun _ =>
+  N'_applys_vheads hs' f &&& (fun hsN' =>
+  hs_match_rec hs hs' 0 &&& (fun _ =>
+  segRLs_rec_v hsN' hs' ws0 T &&& (fun '(res0,res) =>
+  Some (res0,inr ws'::res))))))))
+end.
+
+Definition sideRLs_rec_v hsN' hs '(ws,w) T :=
+segRLs_rec_v hsN' hs ws T &&& (fun '(hsN',hs,ws0) =>
+let hs:=vheads_v hs 0 (fun _=>true) in
+N'_match_vheads hs hsN' &&& (fun f =>
+N'_matched_vheads hs hsN' f &&& (fun _ =>
+sideRLs_rec hs [] w T &&& (fun '(ws1,w0) =>
+Some (ws0++[inl ws1],w0))))).
+
+Definition vseg_eval n (w:vseg) :=
+match w with
+| inl w => concat w
+| inr w => (concat w)^^n
+end.
+
+Definition vsegs_eval n ws :=
+  flat_map (vseg_eval n) ws.
+
+Definition vside_eval(n:nat)(x:vside) :=
+let '(ws,w):=x in
+(vsegs_eval n ws) *> w *> 0inf.
+
+Definition vseg_O (w:vseg) :=
+match w with
+| inl w => w
+| inr w => []
+end.
+
+Definition vseg_S (w:vseg) :=
+match w with
+| inl w => [inl w]
+| inr w => [inl w;inr w]
+end.
+
+Definition vside_S (x:vside) :=
+let '(ws,w):=x in
+(flat_map vseg_S ws,w).
+
+Definition vside_O (x:vside) :=
+let '(ws,w):=x in
+(flat_map vseg_O ws,w).
+
+Fixpoint vsegs_rot0 (w:list seg) (ws:list vseg): list vseg :=
+match ws,w with
+| inl [w']::ws',w0::w1 =>
+  if eqb w0 w' then
+    inl [w0] :: vsegs_rot0 (w1++[w0]) ws'
+  else
+    inr w :: ws
+| _,_ => inr w :: ws
+end.
+
+Fixpoint vsegs_rot(ws:list vseg) :=
+match ws with
+| w::ws =>
+  let ws:=vsegs_rot ws in
+  match w with
+  | inl w => map (fun w => inl [w]) w ++ ws
+  | inr w => vsegs_rot0 w ws
+  end
+| [] => []
+end.
+
+Definition vside_rot(x:vside) :=
+let '(ws,w):=x in (vsegs_rot ws,w).
+
+Ltac rw_app :=
+  repeat (cbn in * ||
+  rewrite app_nil_r in * ||
+  rewrite concat_app in * ||
+  rewrite flat_map_app in * ||
+  rewrite <-app_assoc in *);
+  trivial;
+  try congruence.
+
+Lemma vside_O_spec x:
+  to_side (vside_O x) = vside_eval 0 x.
+Proof.
+  destruct x as [ws w].
+  cbn.
+  f_equal.
+  clear.
+  unfold vsegs_eval.
+  induction ws; rw_app.
+  f_equal.
+  2: apply IHws.
+  destruct a; rw_app.
+Qed.
+
+Lemma vside_S_spec x n:
+  vside_eval n (vside_S x) = vside_eval (S n) x.
+Proof.
+  destruct x as [ws w].
+  cbn.
+  f_equal.
+  clear.
+  unfold vsegs_eval.
+  induction ws; rw_app.
+  rewrite IHws.
+  destruct a; rw_app.
+Qed.
+
+Lemma vsegs_rot0_spec w ws n:
+  vsegs_eval n (vsegs_rot0 w ws) = vsegs_eval n (inr w::ws).
+Proof with trivial.
+  gen w.
+  induction ws; cbn[vsegs_rot0]; intros...
+  destruct a...
+  destruct l...
+  destruct l0...
+  destruct w...
+  destruct (eqb_spec l0 l)...
+  subst.
+  unfold vsegs_eval in *.
+  cbn[flat_map] in *.
+  rewrite IHws.
+  do 2 rewrite app_assoc.
+  f_equal.
+  unfold vseg_eval.
+  clear.
+  induction n; rw_app.
+Qed.
+
+Lemma vsegs_rot_spec x n:
+  vsegs_eval n (vsegs_rot x) = vsegs_eval n x.
+Proof.
+  induction x; cbn[vsegs_rot].
+  - trivial.
+  - destruct a.
+    + unfold vsegs_eval in *; cbn[flat_map] in *.
+      rewrite flat_map_app.
+      rewrite IHx.
+      f_equal.
+      clear.
+      unfold vseg_eval.
+      induction l; rw_app.
+    + rewrite vsegs_rot0_spec.
+      unfold vsegs_eval in *; rw_app.
+Qed.
+
+Lemma vside_rot_spec x n:
+  vside_eval n (vside_rot x) = vside_eval n x.
+Proof.
+  destruct x as [ws w].
+  cbn.
+  rewrite vsegs_rot_spec.
+  trivial.
+Qed.
+
+Fixpoint N'_heads_eval hs n :=
+match hs with
+| [] => []
+| N'_head_mk h n'::hs => [h]^^(N.to_nat (toN n n')) ++ N'_heads_eval hs n
+end.
+
+Definition f_eval (f:N->option N') i n :=
+match f n with
+| Some n' => toN i n'
+| None => 0
+end.
+
+Lemma N'_apply_vheads_spec hs f i hsN':
+  N'_apply_vheads hs f = Some hsN' ->
+  vheads_eval (f_eval f i) hs (N'_heads_eval hsN' i).
+Proof.
+  gen hsN'.
+  induction hs; cbn[N'_apply_vheads]; intros.
+  - inverts H.
+    ec.
+  - destruct a.
+    des_if' H.
+    cbn in H.
+    destruct n'.
+    + des_if' H.
+      des_if' H.
+      inverts H.
+      cbn.
+      ec.
+      2: eauto 2.
+      eapply N'_Nmap_apply_spec in E1.
+      ec.
+      ec.
+      unfold f_eval.
+      rewrite E0.
+      eauto 1.
+    + inverts H.
+      cbn.
+      ec.
+      2: eauto 2.
+      ec.
+      ec.
+Qed.
+
+Lemma N'_applys_vheads_spec hs f i hsN':
+  N'_applys_vheads hs f = Some hsN' ->
+  vheads_evaln (f_eval f i) hs (N'_heads_eval hsN' i) i.
+Proof.
+  gen hsN'.
+  induction hs; cbn[N'_applys_vheads]; intros.
+  - inverts H.
+    ec.
+  - destruct a.
+    des_if' H.
+    cbn in H.
+    destruct n'.
+    + des_if' H.
+      des_if' H.
+      inverts H.
+      cbn.
+      ec.
+      2: eauto 2.
+      eapply N'_Nmap_applys_spec in E1.
+      ec.
+      ec.
+      unfold f_eval.
+      rewrite E0.
+      eauto 1.
+    + inverts H.
+      cbn.
+      ec.
+      2: eauto 2.
+      ec.
+      ec.
+Qed.
+
+Local Opaque N'_Eqb.
+
+Lemma Nmap_is_id_spec mp u:
+  Nmap_is_id mp = Some u ->
+  mp = Nmap_mk 0 0 0 0.
+Proof.
+  unfold Nmap_is_id.
+  intros.
+  destruct mp; [|inverts H].
+  destruct a0; [|inverts H].
+  destruct a1; [|inverts H].
+  destruct b0; [|inverts H].
+  destruct b1; [|inverts H].
+  ec.
+Qed.
+
+Local Opaque N.add N.mul.
+
+Lemma N'_matched_vheads_spec hs hsN' f n hsv:
+  N'_matched_vheads hs hsN' f = Some tt ->
+  vheads_eval (f_eval f n) hs hsv ->
+  N'_heads_eval hsN' n = hsv.
+Proof.
+  gen hsN' hsv.
+  induction hs; cbn[N'_matched_vheads]; intros.
+  - destruct hsN'; inverts H.
+    inverts H0.
+    ec.
+  - destruct a.
+    destruct hsN' as [|[h'0 h'] hsN'].
+    1: inverts H.
+    des_if' H.
+    des_if' H.
+    cbn in H.
+    destruct n'.
+    + des_if' H.
+      des_if' H.
+      inverts H.
+      des_N_op.
+      inverts H0.
+      destruct u0.
+      cbn.
+      f_equal.
+      2: eauto 2.
+      inverts H2.
+      inverts H5.
+      f_equal.
+      f_equal.
+      apply Nmap_is_id_spec in E1; subst.
+      inverts H2.
+      replace (1*n1+0) with n1 in H by lia.
+      subst n1.
+      unfold f_eval.
+      rewrite E2.
+      lia.
+    + destruct u0.
+      des_N_op.
+      eapply N'_eq_c_spec in H.
+      cbn.
+      rewrite H.
+      inverts H0.
+      f_equal.
+      2: eauto 2.
+      inverts H3.
+      inverts H6.
+      trivial.
+Qed.
+
+Inductive hs_match: (list vhead)->(list vhead)->N->Prop :=
+| hs_match_O id': hs_match [] [] id'
+| hs_match_Sv h n n' hs hs' id mp id':
+  hs_match hs hs' (1+id) ->
+  id'<=id ->
+  hs_match (vhead_mk h n (vN_v id (Nmap_mk 0 0 0 0))::hs) (vhead_mk h n' (vN_v id mp)::hs') id'
+| hs_match_Sc h n n0 n' hs hs' id':
+  hs_match hs hs' id' ->
+  hs_match (vhead_mk h n (vN_c n0)::hs) (vhead_mk h n' (vN_c n0)::hs') id'.
+
+Lemma hs_match_rec_spec hs hs' id0:
+  hs_match_rec hs hs' id0 = Some tt ->
+  hs_match hs hs' id0.
+Proof with (try congruence).
+  gen hs' id0.
+  induction hs; cbn[hs_match_rec]; intros.
+  - destruct hs'; inverts H.
+    ec.
+  - destruct a.
+    destruct n'.
+    + destruct hs' as [|h' hs']...
+      destruct h'...
+      destruct n'...
+      do 4 des_if' H.
+      cbn in H.
+      apply IHhs in H.
+      destruct (eqb_spec h h0); inverts E; subst.
+      destruct (eqb_spec id id1); inverts E0; subst.
+      destruct (N.leb_spec id0 id1); inverts E1; subst.
+      eapply Nmap_is_id_spec in E2; subst.
+      ec; eauto 1.
+    + destruct hs' as [|h' hs']...
+      destruct h'...
+      destruct n'...
+      do 2 des_if' H.
+      cbn in H.
+      apply IHhs in H.
+      destruct (eqb_spec h h0); inverts E; subst.
+      destruct (eqb_spec c c1); inverts E0; subst.
+      ec; eauto 1.
+Qed.
+
+Lemma hs_match_hs'_ge hs hs' id' hs'v i ctx1 ctx2:
+  hs_match hs hs' id' ->
+  (forall i, id'<=i -> ctx1 i = ctx2 i) ->
+  vheads_evaln ctx1 hs' hs'v i ->
+  vheads_evaln ctx2 hs' hs'v i.
+Proof.
+  intro H.
+  gen hs'v i ctx1 ctx2.
+  induction H; intros.
+  - inverts H0.
+    ec.
+  - inverts H2.
+    inverts H5.
+    inverts H9.
+    ec.
+    + ec.
+      ec.
+      rewrite H1 in H6; auto 1.
+    + eapply IHhs_match.
+      2: eauto 1.
+      intros.
+      apply H1; lia.
+  - inverts H1.
+    inverts H4.
+    inverts H8.
+    ec.
+    + ec.
+      ec.
+    + eauto 2.
+Qed.
+
+Lemma hs_match_hs_ge hs hs' id' hsv ctx1 ctx2:
+  hs_match hs hs' id' ->
+  (forall i, id'<=i -> ctx1 i = ctx2 i) ->
+  vheads_eval ctx1 hs hsv ->
+  vheads_eval ctx2 hs hsv.
+Proof.
+  intro H.
+  gen hsv ctx1 ctx2.
+  induction H; intros.
+  - inverts H0.
+    ec.
+  - inverts H2.
+    inverts H5.
+    inverts H8.
+    ec.
+    + ec.
+      ec.
+      rewrite H1 in H5; auto 1.
+    + eapply IHhs_match.
+      2: eauto 1.
+      intros.
+      apply H1; lia.
+  - inverts H1.
+    inverts H4.
+    inverts H7.
+    ec.
+    + ec.
+      ec.
+    + eauto 2.
+Qed.
+
+Lemma hs_match_spec1 hs hs' id':
+  hs_match hs hs' id' ->
+  forall ctx hs'v i,
+  vheads_evaln ctx hs' hs'v (N.succ i) ->
+  exists ctx',
+  (vheads_evaln ctx' hs' hs'v i /\
+  (forall hsv, vheads_eval ctx' hs hsv -> vheads_eval ctx hs' hsv)).
+Proof.
+  intro H.
+  induction H; intros.
+  - inverts H.
+    eexists ctx; split.
+    1: ec.
+    intros.
+    inverts H.
+    ec.
+  - inverts H1.
+    eapply IHhs_match in H7.
+    destruct H7 as [ctx' [I1 I2]].
+    inverts H4.
+    inverts H7.
+    inverts H5.
+    1: lia.
+    replace k with i in * by lia.
+    exists (fun x => if x=?id then n1 else ctx' x); split.
+    + ec.
+      2: {
+        eapply hs_match_hs'_ge; eauto 1.
+        intros.
+        destruct (N.eqb_spec i0 id); lia.
+      }
+      ec.
+      ec.
+      destruct (N.eqb_spec id id); [eauto 1|lia].
+    + intros.
+      inverts H3.
+      inverts H6.
+      inverts H10.
+      inverts H6.
+      destruct (N.eqb_spec id id); [|lia].
+      subst.
+      ec.
+      * ec.
+        ec.
+        eauto 1.
+      * eapply I2.
+        eapply hs_match_hs_ge.
+        3: apply H9.
+        1: eauto 1.
+        intros.
+        cbn.
+        destruct (N.eqb_spec i0 id); lia.
+  - inverts H0.
+    eapply IHhs_match in H6.
+    destruct H6 as [ctx' [I1 I2]].
+    inverts H3.
+    inverts H6.
+    exists ctx'; split.
+    + ec.
+      2: eauto 1.
+      ec.
+      ec.
+    + intros.
+      inverts H0.
+      inverts H3.
+      inverts H6.
+      ec.
+      2: eauto 2.
+      ec.
+      ec.
+Qed.
+
+Lemma hs_match_spec2 hs hs' id':
+  hs_match hs hs' id' ->
+  forall ctx hs'v,
+  vheads_evaln ctx hs' hs'v 0 ->
+  vheads_eval ctx hs hs'v.
+Proof.
+  intro H.
+  induction H; intros.
+  - inverts H.
+    ec.
+  - inverts H1.
+    inverts H4.
+    inverts H8.
+    ec.
+    2: eauto 2.
+    ec.
+    ec.
+    inverts H5.
+    + applys_eq (Nmap_apply_mk 0 0 0 0 (ctx id)); lia.
+    + lia.
+  - inverts H0.
+    inverts H3.
+    inverts H7.
+    ec.
+    2: eauto 2.
+    ec.
+    ec.
+Qed.
+
+Lemma segRLs_rec'_specn hs ws T hs' ws' i:
+  segRLs_rec' hs ws T = Some (hs',ws') ->
+  hs_match hs hs' 0 ->
+  forall ctx hs'v,
+  vheads_evaln ctx hs' hs'v i ->
+  exists hsv,
+  vheads_eval ctx hs hsv /\
+  segRLs tm hsv hs'v ((concat ws)^^(N.to_nat i)) ((concat ws')^^(N.to_nat i)).
+Proof.
+  intros H H0.
+  induction i using N.peano_ind; intros.
+  - exists hs'v; split.
+    + eapply hs_match_spec2 in H0; eauto 1.
+    + apply segRLs_nil.
+  - replace (N.to_nat (N.succ i)) with (S (N.to_nat i))%nat by lia.
+    cbn[lpow].
+    eapply hs_match_spec1 in H0.
+    2: eauto 1.
+    destruct H0 as [ctx' [X1 X2]].
+    apply IHi in X1.
+    destruct X1 as [hsv [X1a X1b]].
+    specialize (X2 _ X1a).
+    eapply segRLs_rec'_spec in X2.
+    2: eauto 1.
+    destruct X2 as [hsv0 [I1 I2]].
+    eexists; split.
+    1: eauto 1.
+    eapply segRLs_concat; eauto 1.
+Qed.
+
+
+Lemma segRLs_rec_v_spec hsN' hs ws T hsN'0 hs' ws' n:
+  segRLs_rec_v hsN' hs ws T = Some (hsN'0,hs',ws') ->
+  segRLs tm (N'_heads_eval hsN' n) (N'_heads_eval hsN'0 n) (vsegs_eval (N.to_nat n) ws) (vsegs_eval (N.to_nat n) ws').
+Proof.
+  gen hsN' hs hsN'0 hs' ws'.
+  induction ws; cbn[segRLs_rec_v]; intros.
+  - inverts H.
+    apply segRLs_nil.
+  - destruct a.
+    + des_if' H.
+      destruct p as [hs'0 ws'0].
+      des_if' H.
+      destruct p as [hs'1 ws'1].
+      des_if' H.
+      des_if' H.
+      des_if' H.
+      des_if' H.
+      destruct p as [[res1 res0] res].
+      inverts H.
+      unfold vsegs_eval; cbn.
+      eapply segRLs_concat.
+      2: eapply IHws; eauto 1.
+      eapply N'_apply_vheads_spec in E3.
+      eapply segRLs_rec'_spec in E0.
+      2: eauto 1.
+      destruct E0 as [hsv [E0a E0b]].
+      applys_eq E0b.
+      destruct u.
+      eapply N'_matched_vheads_spec in E2; eauto 1.
+    + des_if' H.
+      destruct p as [hs'0 ws'0].
+      des_if' H.
+      destruct p as [hs'1 ws'1].
+      des_if' H.
+      des_if' H.
+      des_if' H.
+      des_if' H.
+      des_if' H.
+      destruct u0.
+      destruct p as [[res1 res0] res].
+      inverts H.
+      unfold vsegs_eval; cbn.
+      eapply segRLs_concat.
+      2: eapply IHws; eauto 1.
+      eapply N'_applys_vheads_spec in E3.
+      eapply hs_match_rec_spec in E4.
+      eapply segRLs_rec'_specn in E0.
+      2,3: eauto 1.
+      destruct E0 as [hsv [E0a E0b]].
+      applys_eq E0b.
+      destruct u.
+      eapply N'_matched_vheads_spec in E2; eauto 1.
+Qed.
+
+Lemma sideRLs_rec_v_spec hsN' hs ws T ws' n:
+  sideRLs_rec_v hsN' hs ws T = Some (ws') ->
+  sideRLs tm (N'_heads_eval hsN' n) (vside_eval (N.to_nat n) ws) (vside_eval (N.to_nat n) ws').
+Proof.
+  unfold sideRLs_rec_v.
+  intros.
+  destruct ws as [ws w].
+  des_if' H.
+  cbn in H.
+  destruct p as [[hsN'0 hs0] ws0].
+  des_if' H.
+  des_if' H.
+  des_if' H.
+  cbn in H.
+  destruct p as [ws1 w1].
+  destruct u.
+  inverts H.
+  unfold vside_eval.
+  eapply segRLs_rec_v_spec in E.
+  unfold vsegs_eval in *.
+  rewrite flat_map_app,Str_app_assoc.
+  eapply segRLs_sideRLs_concat.
+  1: eauto 1.
+  eapply sideRLs_rec_spec in E2.
+  destruct E2 as [hs' [E1a E1b]].
+  unfold to_side in *.
+  eapply N'_matched_vheads_spec in E1.
+  2: eauto.
+  rewrite E1.
+  rw_app.
+Qed.
+
+Section sim_sec.
+Hypothesis hs_step: list head.
+Hypothesis ws_init: (list seg)*seg.
+
+Definition mstep '(ws,w) T :=
+  sideRLs_rec (map (fun h => vhead_c h 1) hs_step) ws w T.
+
+Fixpoint msteps n ws T :=
+match n with
+| O => Some ws
+| S n => mstep ws T &&& (fun ws => msteps n ws T)
+end.
+
+Lemma mstep_spec ws T ws':
+  mstep ws T = Some ws' ->
+  sideRLs tm hs_step (to_side ws) (to_side ws').
+Proof.
+  unfold mstep.
+  intros.
+  destruct ws as [ws w].
+  eapply sideRLs_rec_spec with (ctx:=fun _=>0) in H.
+  destruct H as [hs' [I1 I2]].
+  apply vheads_c_spec in I1.
+  subst.
+  apply I2.
+Qed.
+
+Definition hR: DH0 := fst (hd ((q0,[]),(q0,[])) hs_step).
+Definition hs_step' := snd (rcons hs_step hR).
+Hypothesis hs_step'_spec:
+  lcons hR hs_step' = (hs_step,hR).
+Hypothesis hs_step'_ne: hs_step' <> [].
+
+Hypothesis lh: side.
+Hypothesis lh_spec:
+  sideRLs (flip tm) hs_step' lh lh.
+
+Definition S' x :=
+  lh {{{ (hR,R) }}} to_side x.
+
+Definition S'' x :=
+  lh {{{ (hR,R) }}} x.
+
+Hypothesis init:
+  c0 -[ tm ]->* S' ws_init.
+
+Lemma BigStep ws ws':
+  sideRLs tm hs_step (ws) (ws') ->
+  S'' ws -[ tm ]->+ S'' ws'.
+Proof.
+  intros H.
+  apply (sideRLs_concat_v2 hs_step'_spec hs_step'_ne lh_spec H).
+Qed.
+
+Definition decide_nonhalt pp T :=
+  msteps pp ws_init T &&& (fun x0 =>
+  mstep x0 T &&& (fun x1 =>
+  mstep x1 T &&& (fun x2 =>
+  interpolate' x0 x1 x2 T &&& (fun x =>
+  sideRLs_rec_v (map (fun h => (N'_head_mk h (N'_c 1))) hs_step) (map (fun h => vhead_c h 1) hs_step) x T &&& (fun x' =>
+  b2o (eqb (vside_O x) x0) &&& (fun _ =>
+  b2o (eqb (vside_rot (vside_S x)) (vside_rot x')) &&& (fun _ =>
+  Some tt
+  ))))))).
+
+Lemma msteps_spec n x T x':
+  msteps n x T = Some x' ->
+  S' x -[ tm ]->* S' x'.
+Proof.
+  gen x x'.
+  induction n; cbn[msteps]; intros.
+  - inverts H.
+    finish.
+  - des_if' H.
+    inverts H.
+    apply mstep_spec in E.
+    apply BigStep in E.
+    apply IHn in H1.
+    follow100 E.
+    apply H1.
+Qed.
+
+Lemma N'_heads_eval_c_spec hs i:
+  hs = N'_heads_eval (map (fun h : head => N'_head_mk h (N'_c 1)) hs) i.
+Proof.
+  induction hs; intros.
+  - trivial.
+  - cbn.
+    rewrite <-IHhs.
+    reflexivity.
+Qed.
+
+Lemma decide_nonhalt_spec pp T:
+  decide_nonhalt pp T = Some tt ->
+  ~halts tm c0.
+Proof.
+  unfold decide_nonhalt.
+  intros.
+  do 7 des_if' H.
+  inverts H.
+  apply msteps_spec in E.
+  destruct (eqb_spec (vside_O p2) p); inverts E4; subst.
+  destruct (eqb_spec (vside_rot (vside_S p2)) (vside_rot p3)); inverts E5; subst.
+  eapply multistep_nonhalt.
+  1: follow init; apply E.
+  change (S' (vside_O p2)) with (S'' (to_side (vside_O p2))).
+  eapply progress_nonhalt_cond with (P:=fun x => exists i, x=vside_eval i p2).
+  2: exists O; apply vside_O_spec.
+  intros x [i0 HP].
+  eexists; split.
+  2: exists (S i0); reflexivity.
+  apply BigStep.
+  subst.
+  eapply sideRLs_rec_v_spec with (n:=N.of_nat i0) in E3.
+  rewrite Nnat.Nat2N.id in E3.
+  rewrite <-vside_S_spec.
+  rewrite <-(vside_rot_spec (vside_S _)).
+  rewrite e.
+  rewrite vside_rot_spec.
+  applys_eq E3.
+  apply N'_heads_eval_c_spec.
+Qed.
+
+End sim_sec.
+
+End sec.
+
+Require Import String.
+
+Close Scope N.
+
+Ltac des_all H :=
+  repeat
+  match type of H with
+  | match ?a with _ => _ end = _ => destruct a
+  | None = Some _ => inverts H
+  | Some _ = Some _ => inverts H
+  end.
+
+
